Veir/Dialects/LLVM/OpInfo.lean
@@ -26,18 +26,44 @@ match op with
 | .icmp => IcmpProperties
 | .cond_br => CondBrProperties
 | .alloca => AllocaProperties
-| .load => LoadProperties
-| .store => StoreProperties
-| .getelementptr => GetelementptrProperties
+| .load => LoadProperties -- attribute
+| .store => StoreProperties -- attribute
+| .getelementptr => GetelementptrProperties -- attribute
 | .fadd | .fsub | .fmul | .fdiv | .frem => FastMathFlagsProperties
 | .func => LLVMFuncProperties
 | .module_flags => LLVMModuleFlagsProperties
 | _ => Unit
 
+def Llvm.propertySize (op : Llvm) : UInt64 :=
+match op with
+| .mlir__constant => 8
+| .add => 1
+| .sub => 1
+| .mul => 1
+| .udiv => 1
+| .sdiv => 1
+| .shl => 1
+| .lshr => 1
+| .ashr => 1
+| .or => 1
+| .trunc => 1
+| .zext => 1
+| .icmp => 1
+| .cond_br => 8 -- attribute
+| .alloca => 8 -- attribute
+| .load => 8 -- attribute
+| .store => 8 -- attribute
+| .getelementptr => 8 -- attribute
+| .fadd | .fsub | .fmul | .fdiv | .frem => 1
+| .func => 8
+| .module_flags => 8
+| _ => 0
+
+
 instance : HasDialectOpInfo Llvm where
   propertiesOf := Llvm.propertiesOf
-  propertySize _ := 4
-  propertySize_small {op} := by grind
+  propertySize op := Llvm.propertySize op
+  propertySize_small {op} := by cases op <;> simp [Llvm.propertySize]
 
 end
 
